src/use_cases/assign_mcl/defs.lean
@@ -24,7 +24,7 @@ lemma tid_is_tlocal : is_tlocal (sig.val "tid") := by apply eq.refl
 -- TODO generate those proofs directly from signature
 -- make type classes out of those
 -- make name explicit in state.update
-def read_tid := (expression.tlocal_var "tid" (λ_, 0) (show type_of (sig.val "tid") = type.int, by apply eq.refl) (show (sig.val "tid").type.dim = 1, by apply eq.refl) tid_is_tlocal)
+def read_tid := (expression.tlocal_var "tid" (λ_, 0) tid_is_tlocal)
 
 instance : has_one (expression sig (type_of (sig.val "b"))) := begin
     have : type_of (sig.val "b") = type.int := by apply eq.refl,
@@ -34,11 +34,11 @@ end
 
 def p₁ : mclp sig := mclp.intro (λ m, 100) (
     mclk.shared_assign "a" v[read_tid] (by refl) (by refl) read_tid ;;
-    mclk.shared_assign "b" v[read_tid] (by refl) (by refl) (read_tid + (expression.literal_int 1 (by refl)))
+    mclk.shared_assign "b" v[read_tid] (by refl) (by refl) (read_tid + (expression.literal_int 1))
 )
 
 def p₂ : mclp sig := mclp.intro (λ m, 100) (
-    mclk.shared_assign "b" v[read_tid] (by refl) (by refl) (read_tid + (expression.literal_int 1 (by refl))) ;;
+    mclk.shared_assign "b" v[read_tid] (by refl) (by refl) (read_tid + (expression.literal_int 1)) ;;
     mclk.shared_assign "a" v[read_tid] (by refl) (by refl) read_tid
 )
 
