src/use_cases/coarsening/defs.lean
@@ -1,0 +1,131 @@
+import mcl
+import parlang.lemmas_memory
+
+open mcl
+
+namespace coarsening
+
+def sigc : signature_core
+| "tid" := { scope := scope.tlocal, type := ⟨1, type.int⟩ }
+| "i" := { scope := scope.tlocal, type := ⟨1, type.int⟩ }
+| "j" := { scope := scope.tlocal, type := ⟨1, type.int⟩ }
+| _ := { scope := scope.shared, type := ⟨1, type.float⟩ }
+
+def sig : signature := ⟨sigc, ⟨rfl, rfl, rfl⟩⟩
+
+open mcl.expression
+open parlang
+
+/-- Copies the *j*-th element from a to b -/
+def copy : mclk sig := mclk.shared_assign "b" v[@tlocal_var sig "j" (λ_, 0) rfl] rfl rfl (@shared_var sig "a" (v[@tlocal_var sig "j" (λ_, 0) rfl]).nth rfl)
+
+def e₁ := 10
+def f₁ := 10
+def p₁ : mclp sig := mclp.intro (λ m, e₁) (
+    mclk.for "i" rfl rfl (literal_int 0) (@tlocal_var sig "i" (λ_, 0) rfl < literal_int f₁) (mclk.tlocal_assign "i" v[0] rfl rfl $ tlocal_var "i" (λ_, 0) rfl + literal_int 1) (
+        mclk.tlocal_assign "j" v[literal_int 0] rfl rfl (@tlocal_var sig "tid" (λ_, 0) rfl * literal_int e₁ + @tlocal_var sig "i" (λ_, 0) rfl) ;;
+        copy
+    )
+)
+
+def e₂ := 5
+def f₂ := 20
+def p₂ : mclp sig := mclp.intro (λ m, e₂) (
+    mclk.for "i" rfl rfl (literal_int 0) (@tlocal_var sig "i" (λ_, 0) rfl < literal_int f₂) (mclk.tlocal_assign "i" v[0] rfl rfl $ @tlocal_var sig "i" (λ_, 0) rfl + literal_int 1) (
+        mclk.tlocal_assign "j" v[literal_int 0] rfl rfl (@tlocal_var sig "tid" (λ_, 0) rfl * literal_int e₂ + @tlocal_var sig "i" (λ_, 0) rfl) ;;
+        copy
+    )
+)
+
+def read_tid {sig : signature} := @tlocal_var sig "tid" (λ_, 0) sig.property.right.right
+
+def coarsen_kernel_assertion {sig : signature}
+(P : memory (parlang_mcl_shared sig) → memory (parlang_mcl_shared sig) → Prop)
+(f₁ : memory (parlang_mcl_shared sig) → ℕ) (f₂ : memory (parlang_mcl_shared sig) → ℕ) 
+(m₁ : memory (parlang_mcl_shared sig)) (m₂ : memory (parlang_mcl_shared sig)) 
+(n₁) (s₁ : state n₁ (memory $ parlang_mcl_tlocal sig) $ parlang_mcl_shared sig) 
+(ac₁ : vector bool n₁) (n₂) (s₂ : state n₂ (memory $ parlang_mcl_tlocal sig) $ parlang_mcl_shared sig) 
+(ac₂ : vector bool n₂) := 
+s₁.syncable m₁ ∧ s₂.syncable m₂ ∧ n₁ = f₁ m₁ ∧ n₂ = f₂ m₂ ∧
+(∀ i : fin n₁, s₁.threads.nth i = { tlocal := mcl_init i, shared := m₁, stores := ∅, loads := ∅ }) ∧ 
+(∀ i : fin n₂, s₂.threads.nth i = { tlocal := mcl_init i, shared := m₂, stores := ∅, loads := ∅ }) ∧
+P m₁ m₂ ∧ all_threads_active ac₁ ∧ all_threads_active ac₂
+
+/-- only works with constant number of threads -/
+theorem coarsen (e₁ e₂) 
+(sig) (k₁ : mclk sig) (k₂ : mclk sig) (h₁ : type_of (sig.val "k") = type.int) (h₂ : ((sig.val "k").type).dim = 1) (h₃) (Q : parlang.memory (parlang_mcl_shared sig) → parlang.memory (parlang_mcl_shared sig) → Prop)
+(h : rhl.mclk_rel (λn₁ (s₁ : state n₁ (memory (parlang_mcl_tlocal sig)) (parlang_mcl_shared sig)) ac₁ n₂ s₂ ac₂, ∃ m₁ m₂, 
+parlang.initial_kernel_assertion mcl_init mcl_init eq (λm, e₁) (λm, e₂) m₁ m₂ n₁ 
+(s₁.map_active_threads ac₁ $ λts, ts.compute $ λm, m.update ⟨"k", by rw h₂; exact v[0]⟩ (eq.mpr (show _ = ℕ, from begin unfold parlang_mcl_tlocal, simp, unfold signature.lean_type_of lean_type_of, rw h₁, end) 0)) ac₁ n₂ 
+(s₂.map_active_threads ac₂ $ λts, ts.compute $ λm, m.update ⟨"k", by rw h₂; exact v[0]⟩ (eq.mpr (show _ = ℕ, from begin unfold parlang_mcl_tlocal, simp, unfold signature.lean_type_of lean_type_of, rw h₁, end) 0)) ac₂)
+    k₁ k₂ 
+  (λn₁ s₁ ac₁ n₂ s₂ ac₂, ∃ m₁ m₂, s₁.syncable m₁ ∧ s₂.syncable m₂ ∧ Q m₁ m₂)) :
+rhl.mclp_rel eq 
+(mclp.intro (λ m, e₁) (
+    @mclk.tlocal_assign sig type.int _ "k" v[literal_int 0] h₁ h₂ read_tid ;;
+    k₁
+))
+(mclp.intro (λ m, e₂) (
+    mclk.for "k" h₁ h₂ read_tid ((by rw ← h₁; exact @tlocal_var sig "k" (λ_, 0) h₃) < literal_int e₂) (mclk.tlocal_assign "k" v[0] h₁ h₂ $ tlocal_var "k" (λ_, 0) h₃ + literal_int e₂)
+        k₂
+)) Q := begin
+    apply rhl.rel_mclk_to_mclp,
+    intros n₁ n₂ s₁ s₁' s₂ ac₁ ac₂ hp he₁,
+    cases hp with m₁ hp,
+    cases hp with m₂ hp,
+    specialize h n₁ n₂ (state.map_active_threads ac₁ (thread_state.compute $ λm, m.update ⟨"k", by rw h₂; exact v[0]⟩ (eq.mpr _ $ m.get ⟨"tid", begin rw sig.property.right.left, exact v[0], end⟩)) s₁) s₁' s₂ ac₁ ac₂,
+    swap 2, {
+        unfold parlang_mcl_tlocal signature.lean_type_of lean_type_of,
+        rw h₁,
+        rw sig.property.left,
+    },
+    specialize h _,
+    swap 2,
+    {
+        use m₁,
+        use m₂,
+        unfold initial_kernel_assertion,
+        unfold initial_kernel_assertion at hp,
+        delta thread_state.compute,
+        rw ← state.syncable_tlocal,
+        rw ← state.syncable_tlocal,
+        rw ← state.syncable_tlocal,
+        split, {
+            exact hp.left,
+        },
+        split, {
+            exact hp.right.left,
+        },
+        split, {
+            exact hp.right.right.left,
+        },
+        split, {
+            exact hp.right.right.right.left,
+        },
+        split, {
+            intros i,
+            have : vector.nth ac₁ i = tt := sorry,
+            simp only [state.map_active_threads_nth_ac this],
+            rw memory.update_update_eq,
+            rw hp.right.right.right.right.left i,
+            simp [mcl_init],
+            funext i,
+            cases i,
+            by_cases a : i_fst = "k",
+            {
+                subst a,
+                sorry,
+            },
+            sorry,
+        },
+        sorry,
+    },
+    sorry,
+end
+
+example : rhl.mclp_rel eq p₁ p₂ eq := begin 
+    sorry,
+    -- apply main transformation rule
+end
+
+end coarsening
